theories/lang/steps_access.v
@@ -7,7 +7,7 @@ Lemma access1_in_stack stk kind t cids n stk' :
    ∃ it, it ∈ stk ∧ it.(tg) = t ∧ it.(perm) ≠ Disabled.
 Proof.
   rewrite /access1. case find_granting as [gip|] eqn:Eq1; [|done].
-  apply fmap_Some in Eq1 as [[i it] [[IN [GR Eq]]%list_find_Some EQ]].
+  apply fmap_Some in Eq1 as [[i it] [(IN & [GR Eq] & FR)%list_find_Some EQ]].
   intros ?. exists it. split; last split; [|done|].
   - by eapply elem_of_list_lookup_2.
   - intros Eq1. by rewrite Eq1 in GR.
@@ -247,8 +247,8 @@ Lemma dealloc1_Some stk t cids :
 Proof.
   rewrite /dealloc1. move => [[]].
   case find_granting eqn:GR; [|done]. simpl.
-  apply fmap_Some_1 in GR as [[i it'] [[GR [? ?]]%list_find_Some ?]]. simplify_eq.
-  rewrite /find_top_active_protector.
+  apply fmap_Some_1 in GR as [[i it'] [(GR & [? ?] &?)%list_find_Some ?]].
+  simplify_eq. rewrite /find_top_active_protector.
   case list_find eqn:EqF; [done|]. intros _.
   apply list_find_None in EqF. exists it'.
   have ?: it' ∈ stk by eapply elem_of_list_lookup_2. done.
